Outer interface proof for the Selection pass

backend/CminorSel.v
@@ -448,21 +448,20 @@ Inductive step: state -> trace -> state -> Prop :=
 
 End RELSEM.
 
-Inductive initial_state (p: program): state -> Prop :=
-  | initial_state_intro: forall b f m0,
+Inductive initial_state (p: program): query li_c -> state -> Prop :=
+  | initial_state_intro: forall id b f vargs m,
       let ge := Genv.globalenv p in
-      Genv.init_mem p = Some m0 ->
-      Genv.find_symbol ge p.(prog_main) = Some b ->
+      Ple (Genv.genv_next ge) (Mem.nextblock m) ->
+      Genv.find_symbol ge (str2ident id) = Some b ->
       Genv.find_funct_ptr ge b = Some f ->
-      funsig f = signature_main ->
-      initial_state p (Callstate f nil Kstop m0).
+      initial_state p (id, funsig f, vargs, m) (Callstate f nil Kstop m).
 
-Inductive final_state: state -> int -> Prop :=
+Inductive final_state: state -> reply li_c -> Prop :=
   | final_state_intro: forall r m,
-      final_state (Returnstate (Vint r) Kstop m) r.
+      final_state (Returnstate r Kstop m) (r, m).
 
 Definition semantics (p: program) :=
-  Semantics step (initial_state p) final_state (Genv.globalenv p).
+  Semantics li_c step (initial_state p) final_state (Genv.globalenv p).
 
 Hint Constructors eval_expr eval_exprlist eval_condexpr: evalexpr.
 
