backend/Selectionproof.v
@@ -1080,37 +1080,44 @@ Proof.
 Qed.
 
 Lemma sel_initial_states:
-  forall S, Cminor.initial_state prog S ->
-  exists R, initial_state tprog R /\ match_states S R.
+  forall w q1 q2, match_query cc_extends_triangle w q1 q2 ->
+  forall S, Cminor.initial_state prog q1 S ->
+  exists R, initial_state tprog q2 R /\ match_states S R.
 Proof.
+  inv_triangle_query.
   destruct 1.
   exploit function_ptr_translated; eauto. intros (cu & f' & A & B & C).
   econstructor; split.
-  econstructor.
-  eapply (Genv.init_mem_match TRANSF); eauto.
-  rewrite (match_program_main TRANSF). fold tge. rewrite symbols_preserved. eauto.
-  eexact A.
-  rewrite <- H2. eapply sig_function_translated; eauto.
+  {
+    erewrite <- sig_function_translated by eauto.
+    econstructor.
+    + fold tge. rewrite genv_next_preserved. assumption.
+    + fold tge. rewrite symbols_preserved. eassumption.
+    + fold tge. assumption.
+  }
   econstructor; eauto. red; intros; constructor. apply Mem.extends_refl.
 Qed.
 
 Lemma sel_final_states:
-  forall S R r,
-  match_states S R -> Cminor.final_state S r -> final_state R r.
+  forall w S R r1, match_states S R -> Cminor.final_state S r1 ->
+  exists r2, match_reply cc_extends_triangle w r1 r2 /\ final_state R r2.
 Proof.
   intros. inv H0. inv H.
+  exists (v', m'). split; eauto using match_reply_cc_extends_triangle.
   apply match_call_cont_cont in MC. destruct MC as (cunit0 & hf0 & MC).
-  inv MC. inv LD. constructor.
+  inv MC. constructor.
 Qed.
 
 Theorem transf_program_correct:
-  forward_simulation cc_extends (Cminor.semantics prog) (CminorSel.semantics tprog).
+  forward_simulation cc_extends cc_extends_triangle
+    (Cminor.semantics prog)
+    (CminorSel.semantics tprog).
 Proof.
-  apply forward_simulation_opt with (match_states := match_states) (measure := measure).
+  apply forward_simulation_opt with (match_states := fun _ => match_states) (measure := measure).
   apply senv_preserved.
   apply sel_initial_states; auto.
   apply sel_final_states; auto.
-  apply sel_step_correct; auto.
+  auto using sel_step_correct.
 Qed.
 
 End PRESERVATION.
